wip

src/Distributions/BernoulliExpNeg/Model.dfy
@@ -5,7 +5,9 @@
 
 module BernoulliExpNeg.Model {
   import Rationals
+  import Rand
   import Uniform
+  import Bernoulli
   import Monad
   import Loops
   import BernoulliModel = Bernoulli.Model
@@ -15,23 +17,35 @@ module BernoulliExpNeg.Model {
     requires gamma.numer >= 0
   {
     Monad.Bind(
-      GammaReductionLoop(gamma),
+      GammaReductionLoop((true, gamma)),
       (bgamma: (bool, Rationals.Rational)) =>
-        if bgamma.0 then
-          SampleGammaLe1(bgamma.1)
-        else
-          Monad.Return(false)
+        var res: Monad.Hurd<bool> :=
+          if bgamma.0 then
+            // This if condition should not be needed, but Monad.Bind does not accept functions with preconditions
+            if 0 <= bgamma.1.numer <= bgamma.1.denom
+            then SampleGammaLe1(bgamma.1)
+            else Monad.Return(false) // return a dummy value because this path should never be taken
+          else
+            Monad.Return(false);
+        res
     )
   }
 
-  ghost function GammaReductionLoop(gamma: Rationals.Rational): Monad.Hurd<(bool, Rationals.Rational)>
-    requires gamma.numer >= 0
+  ghost function GammaReductionLoop(bgamma: (bool, Rationals.Rational)): Monad.Hurd<(bool, Rationals.Rational)>
+    requires bgamma.1.numer >= 0
+    decreases bgamma.1.numer
   {
-    assume {:axiom} false; // assume termination
-    Loops.While(
-      (bgamma: (bool, Rationals.Rational)) => bgamma.0 && bgamma.1.denom <= bgamma.1.numer,
-      GammaReductionLoopIter,
-      (true, gamma)
+    if !bgamma.0 || bgamma.1.numer < bgamma.1.denom
+    then Monad.Return(bgamma)
+    else Monad.Bind(
+      GammaReductionLoopIter(bgamma),
+      (bgamma': (bool, Rationals.Rational)) =>
+        var res: Monad.Hurd<(bool, Rationals.Rational)> :=
+          // This if condition should not be needed, but Monad.Bind does not accept functions with preconditions
+          if bgamma'.1.numer < 0 || bgamma'.1.numer >= bgamma.1.numer
+          then Monad.Return((bgamma'.0, Rationals.Rational(0, 1)))
+          else GammaReductionLoop(bgamma'); // return a dummy value because this path should never be taken
+        res
     )
   }
 
@@ -45,32 +59,75 @@ module BernoulliExpNeg.Model {
   }
 
   ghost function SampleGammaLe1(gamma: Rationals.Rational): Monad.Hurd<bool>
-  {
-    if 0 <= gamma.numer <= gamma.denom
-    then Monad.Bind(
-           GammaLe1Loop(gamma, (true, 0)),
-           (ak: (bool, nat)) => Monad.Return(ak.1 % 2 == 1)
-         )
-    else Monad.Return(false) // to keep this function total, we return a dummy value here
-  }
-
-  ghost function GammaLe1Loop(gamma: Rationals.Rational, ak: (bool, nat)): Monad.Hurd<(bool, nat)>
-    requires 0 <= gamma.numer <= gamma.denom
-  {
-    assume {:axiom} false; // assume termination
-    Loops.While(
-      (ak: (bool, nat)) => ak.0,
-      (ak: (bool, nat)) => GammaLe1LoopIter(gamma, ak),
-      ak
-    )
-  }
-
-  ghost function GammaLe1LoopIter(gamma: Rationals.Rational, ak: (bool, nat)): Monad.Hurd<(bool, nat)>
-    requires 0 <= gamma.numer <= gamma.denom
+  requires 0 <= gamma.numer <= gamma.denom
   {
     Monad.Bind(
-      BernoulliModel.Sample(gamma.numer, (ak.1 + 1) * gamma.denom),
-      (a': bool) => Monad.Return((a', ak.1 + 1))
+      GammaLe1Loop(gamma)((true, 0)),
+      (ak: (bool, nat)) => Monad.Return(ak.1 % 2 == 1)
     )
+  }
+
+  ghost function GammaLe1Loop(gamma: Rationals.Rational): ((bool, nat)) -> Monad.Hurd<(bool, nat)>
+    requires 0 <= gamma.numer <= gamma.denom
+  {
+    (ak: (bool, nat)) =>
+      GammaLe1LoopTerminatesAlmostSurely(gamma);
+      Loops.While(
+        GammaLe1LoopCondition,
+        GammaLe1LoopIter(gamma),
+        ak
+      )
+  }
+
+  ghost function GammaLe1LoopCondition(ak: (bool, nat)): bool {
+    ak.0
+  }
+
+  ghost function GammaLe1LoopIter(gamma: Rationals.Rational): ((bool, nat)) -> Monad.Hurd<(bool, nat)>
+    requires 0 <= gamma.numer <= gamma.denom
+  {
+    (ak: (bool, nat)) =>
+      var res: Monad.Hurd<(bool, nat)> := Monad.Bind(
+        BernoulliModel.Sample(gamma.numer, (ak.1 + 1) * gamma.denom),
+        (a': bool) => Monad.Return((a', ak.1 + 1)));
+      res
+  }
+
+  lemma {:vcs_split_on_every_assert} GammaLe1LoopIterProperty(gamma: Rationals.Rational, a: bool, k: nat, s: Rand.Bitstream, a': bool, k': nat, s': Rand.Bitstream)
+    requires 0 <= gamma.numer <= gamma.denom
+    requires k' == k + 1
+    requires (a' , s') == Bernoulli.Model.Sample(gamma.numer, k' * gamma.denom)(s)
+    ensures ((a', k'), s') == GammaLe1LoopIter(gamma)((a,k))(s)
+  {
+    var (a, s') := Bernoulli.Model.Sample(gamma.numer, k' * gamma.denom)(s);
+    assert GammaLe1LoopIter(gamma)((a, k))(s) == ((a', k'), s');
+    assert Monad.Bind(Bernoulli.Model.Sample(gamma.numer, k' * gamma.denom), a => Monad.Return((a, k')))(s) == ((a, k'), s');
+  }
+
+  lemma {:axiom} GammaLe1LoopTerminatesAlmostSurely(gamma: Rationals.Rational)
+    requires 0 <= gamma.numer <= gamma.denom
+    ensures Loops.WhileTerminatesAlmostSurely(GammaLe1LoopCondition, GammaLe1LoopIter(gamma))
+
+  lemma GammaLe1LoopUnroll(gamma: Rationals.Rational, ak: (bool, nat), s: Rand.Bitstream)
+    requires 0 <= gamma.numer <= gamma.denom
+    requires ak.0
+    ensures GammaLe1Loop(gamma)(ak)(s) == Monad.Bind(GammaLe1LoopIter(gamma)(ak), GammaLe1Loop(gamma))(s)
+  {
+    GammaLe1LoopTerminatesAlmostSurely(gamma);
+    assert Eq: forall ak': (bool, nat), s: Rand.Bitstream ::
+      GammaLe1Loop(gamma)(ak')(s) == Loops.While(GammaLe1LoopCondition, GammaLe1LoopIter(gamma), ak')(s) by {
+        forall ak': (bool, nat), s: Rand.Bitstream ensures GammaLe1Loop(gamma)(ak')(s) == Loops.While(GammaLe1LoopCondition, GammaLe1LoopIter(gamma), ak')(s) {}
+      }
+    calc {
+      GammaLe1Loop(gamma)(ak)(s);
+      Loops.While(GammaLe1LoopCondition, GammaLe1LoopIter(gamma), ak)(s);
+      { Loops.WhileUnroll(GammaLe1LoopCondition, GammaLe1LoopIter(gamma), ak, s); }
+      Monad.Bind(
+        GammaLe1LoopIter(gamma)(ak),
+        (ak': (bool, nat)) => Loops.While(GammaLe1LoopCondition, GammaLe1LoopIter(gamma), ak'))
+      (s);
+      { reveal Eq; }
+      Monad.Bind(GammaLe1LoopIter(gamma)(ak), GammaLe1Loop(gamma))(s);
+    }
   }
 }
