src/Distributions/BernoulliExpNeg/Implementation.dfy
@@ -8,11 +8,12 @@ module BernoulliExpNeg.Implementation {
   import Monad
   import Interface
   import Model
+  import Bernoulli
 
   trait {:termination false} Trait extends Interface.Trait {
 
     // Based on Algorithm 1 in https://arxiv.org/pdf/2004.00010.pdf; unverified
-    method BernoulliExpNegSample(gamma: Rationals.Rational) returns (c: bool)
+    method {:vcs_split_on_every_assert} BernoulliExpNegSample(gamma: Rationals.Rational) returns (c: bool)
       modifies this
       requires gamma.numer >= 0
       decreases *
@@ -23,16 +24,17 @@ module BernoulliExpNeg.Implementation {
       while b && gamma'.numer >= gamma'.denom
         decreases gamma'.numer
         invariant gamma'.numer >= 0
+        invariant Model.GammaReductionLoop((true, gamma))(old(s)) == Model.GammaReductionLoop((b, gamma'))(s)
       {
         b := BernoulliExpNegSampleCaseLe1(Rationals.Int(1));
         gamma' := Rationals.Rational(gamma'.numer - gamma'.denom, gamma'.denom);
       }
       if b {
+        assert 0 <= gamma'.numer < gamma'.denom;
         c:= BernoulliExpNegSampleCaseLe1(gamma');
       } else {
         c := false;
       }
-      assume {:axiom} Monad.Result(c, s) == Model.Sample(gamma)(old(s)); // add later
     }
 
     method BernoulliExpNegSampleCaseLe1(gamma: Rationals.Rational) returns (c: bool)
@@ -41,13 +43,26 @@ module BernoulliExpNeg.Implementation {
       decreases *
       ensures Monad.Result(c, s) == Model.SampleGammaLe1(gamma)(old(s))
     {
-      var k := 0;
+      var k: nat := 0;
       var a := true;
+      ghost var initGamma := gamma;
       while a
         decreases *
+        invariant gamma == initGamma
+        invariant Model.GammaLe1Loop(gamma)((a, k))(s) == Model.GammaLe1Loop(gamma)((true, 0))(old(s))
       {
+        ghost var prevK: nat := k;
+        ghost var prevA := a;
+        ghost var prevS := s;
         k := k + 1;
+        assume gamma.numer < k * gamma.denom;
         a := BernoulliSample(Rationals.Rational(gamma.numer, k * gamma.denom));
+        assert ((a, k), s) == Model.GammaLe1LoopIter(gamma)((prevA, prevK))(prevS) by {
+          Model.GammaLe1LoopIterProperty(gamma, prevA, prevK, prevS, a, k, s);
+        }
+        assert Model.GammaLe1Loop(gamma)((prevA, prevK))(prevS) == Model.GammaLe1Loop(gamma)((a, k))(s) by {
+          Model.GammaLe1LoopUnroll(gamma, (prevA, prevK), prevS);
+        }
       }
       c := k % 2 == 1;
       assume {:axiom} Monad.Result(c, s) == Model.SampleGammaLe1(gamma)(old(s)); // add later
